theories/typing/array_util.v
@@ -3,3 +3,68 @@ Set Default Proof Using "Type".
 
 Notation "l +ₗ[ ty ] i" := (l%L +ₗ Z.of_nat (i%nat * ty.(ty_size))%nat)
   (format "l  +ₗ[ ty ]  i", at level 50, left associativity) : loc_scope.
+
+Section array_util.
+  Context `{!typeG Σ}.
+
+  Lemma ty_share_big_sepL {𝔄} (ty: type 𝔄) E aπl d κ l tid q :
+    ↑lftN ⊆ E → lft_ctx -∗ κ ⊑ ty.(ty_lft) -∗
+    &{κ} ([∗ list] i ↦ aπ ∈ aπl, (l +ₗ[ty] i) ↦∗: ty.(ty_own) aπ d tid) -∗ q.[κ]
+      ={E}=∗ |={E}▷=>^d |={E}=>
+        ([∗ list] i ↦ aπ ∈ aπl, ty.(ty_shr) aπ d κ tid (l +ₗ[ty] i)) ∗ q.[κ].
+  Proof.
+    iIntros (?) "#LFT #In Bor κ".
+    iMod (bor_big_sepL with "LFT Bor") as "Bors"; [done|].
+    iInduction aπl as [|] "IH" forall (l q)=>/=.
+    { iApply step_fupdN_full_intro. by iFrame. }
+    iDestruct "κ" as "[κ κ₊]". iDestruct "Bors" as "[Bor Bors]".
+    iMod (ty_share with "LFT In Bor κ") as "Toshr"; [done|].
+    setoid_rewrite <-shift_loc_assoc_nat. iMod ("IH" with "κ₊ Bors") as "Toshrs".
+    iCombine "Toshr Toshrs" as "Toshrs". iApply (step_fupdN_wand with "Toshrs").
+    by iIntros "!> [>[$$] >[$$]]".
+  Qed.
+
+  Lemma ty_own_proph_mt_big_sepL_v {𝔄} (ty: type 𝔄) n E (aπl: vec _ n) l d tid κ q :
+    ↑lftN ⊆ E → lft_ctx -∗ κ ⊑ ty.(ty_lft) -∗
+    ([∗ list] i ↦ aπ ∈ aπl, (l +ₗ[ty] i) ↦∗: ty.(ty_own) aπ d tid) -∗ q.[κ]
+      ={E}=∗ |={E}▷=>^d |={E}=> ∃ξl q', ⌜vapply aπl ./ ξl⌝ ∗ q':+[ξl] ∗
+        (q':+[ξl] ={E}=∗
+          ([∗ list] i ↦ aπ ∈ aπl, (l +ₗ[ty] i) ↦∗: ty.(ty_own) aπ d tid) ∗ q.[κ]).
+  Proof.
+    iIntros (?) "#LFT #In ↦tys κ". iInduction aπl as [|] "IH" forall (l q)=>/=.
+    { iApply step_fupdN_full_intro. iIntros "!>!>". iExists [], 1%Qp.
+      iFrame "κ". do 2 (iSplit; [done|]). by iIntros. }
+    iDestruct "κ" as "[κ κ₊]". iDestruct "↦tys" as "[(% & ↦ & ty) ↦tys]".
+    iMod (ty_own_proph with "LFT In ty κ") as "Toty"; [done|].
+    setoid_rewrite <-shift_loc_assoc_nat. iMod ("IH" with "↦tys κ₊") as "To↦tys".
+    iCombine "Toty To↦tys" as "Upd". iApply (step_fupdN_wand with "Upd").
+    iIntros "!> [>(%&%&%& ξl & Toty) >(%&%&%& ζl & To↦tys)] !>".
+    iDestruct (proph_tok_combine with "ξl ζl") as (?) "[ξζl Toξζl]".
+    iExists _, _. iFrame "ξζl". iSplit; [iPureIntro; by apply proph_dep_vcons|].
+    iIntros "ξζl". iDestruct ("Toξζl" with "ξζl") as "[ξl ζl]".
+    iMod ("Toty" with "ξl") as "[?$]". iMod ("To↦tys" with "ζl") as "[$$]".
+    iExists _. by iFrame.
+  Qed.
+
+  Lemma ty_shr_proph_big_sepL_v {𝔄} (ty: type 𝔄) n E (aπl: vec _ n) d κ tid l κ' q :
+    ↑lftN ⊆ E → lft_ctx -∗ κ' ⊑ κ -∗ κ' ⊑ ty.(ty_lft) -∗
+    ([∗ list] i ↦ aπ ∈ aπl, ty.(ty_shr) aπ d κ tid (l +ₗ[ty] i)) -∗ q.[κ']
+      ={E}▷=∗ |={E}▷=>^d |={E}=> ∃ξl q', ⌜vapply aπl ./ ξl⌝ ∗ q':+[ξl] ∗
+        (q':+[ξl] ={E}=∗
+          ([∗ list] i ↦ aπ ∈ aπl, ty.(ty_shr) aπ d κ tid (l +ₗ[ty] i)) ∗ q.[κ']).
+  Proof.
+    iIntros (?) "#LFT #In #In' tys κ'". iInduction aπl as [|] "IH" forall (l q)=>/=.
+    { iApply step_fupdN_full_intro. iIntros "!>!>!>!>". iExists [], 1%Qp.
+      iFrame "κ'". do 2 (iSplit; [done|]). by iIntros. }
+    iDestruct "κ'" as "[κ' κ'₊]". iDestruct "tys" as "[ty tys]".
+    iMod (ty_shr_proph with "LFT In In' ty κ'") as "Toty"; [done|].
+    setoid_rewrite <-shift_loc_assoc_nat. iMod ("IH" with "tys κ'₊") as "Totys".
+    iIntros "!>!>". iCombine "Toty Totys" as "Upd". iApply (step_fupdN_wand with "Upd").
+    iIntros "[>(%&%&%& ξl & Toty) >(%&%&%& ζl & Totys)] !>".
+    iDestruct (proph_tok_combine with "ξl ζl") as (?) "[ξζl Toξζl]".
+    iExists _, _. iFrame "ξζl". iSplit; [iPureIntro; by apply proph_dep_vcons|].
+    iIntros "ξζl". iDestruct ("Toξζl" with "ξζl") as "[ξl ζl]".
+    iMod ("Toty" with "ξl") as "[$$]". by iMod ("Totys" with "ζl") as "[$$]".
+  Qed.
+
+End array_util.
