theories/typing/sum.v
@@ -195,11 +195,11 @@ Section typing.
     move=> ?. have Copy: ∀i, Copy (hnth base tyl i).
     { move=> *. apply (TCHForall_nth _); by [apply _|]. }
     split; [apply _|]. move=>/= ?????? l ?? SubF.
-    iIntros "#LFT (%i &%&->& Bor & ty) Na [κ κ+]".
+    iIntros "#LFT (%i &%&->& Bor & ty) Na [κ κ₊]".
     iMod (frac_bor_acc with "LFT Bor κ") as (q) "[>[↦i ↦pad] Toκ]";
     [solve_ndisj|]. iDestruct "↦pad" as (vl') "[↦pad %]".
-    iMod (copy_shr_acc with "LFT ty Na κ+") as
-      (q' vl) "(Na & ↦ & #ty & Toκ+)"; [done| |].
+    iMod (copy_shr_acc with "LFT ty Na κ₊") as
+      (q' vl) "(Na & ↦ & #ty & Toκ₊)"; [done| |].
     { rewrite <-SubF, <-union_subseteq_r. apply shr_locsE_subseteq. lia. }
     iDestruct (na_own_acc with "Na") as "[$ ToNa]".
     { apply difference_mono_l. trans (shr_locsE (l +ₗ 1) (max_ty_size tyl));
@@ -214,7 +214,7 @@ Section typing.
     { iIntros "!>!>". iExists i, _, vl, vl'. iFrame "ty". iPureIntro.
       do 2 (split; [done|]). rewrite/= app_length Eq. by f_equal. }
     iIntros "!> Na (↦i' & ↦' & ↦pad')". iDestruct ("ToNa" with "Na") as "Na".
-    iMod ("Toκ+" with "Na [$↦ $↦']") as "[$$]". iApply "Toκ".
+    iMod ("Toκ₊" with "Na [$↦ $↦']") as "[$$]". iApply "Toκ".
     iFrame "↦i ↦i'". iExists vl'. by iFrame.
   Qed.
 
