theories/util/vector.v
@@ -58,6 +58,10 @@ Definition vapply {A B n} (fl: vec (B → A) n) (x: B) : vec A n := vmap (.$ x) 
 Fixpoint vfunsep {A B n} : (B → vec A n) → vec (B → A) n :=
   match n with 0 => λ _, [#] | S _ => λ f, (vhd ∘ f) ::: vfunsep (vtl ∘ f) end.
 
+Lemma lapply_vapply {A B n} (fl: vec (B → A) n) :
+  lapply (vec_to_list fl) = vec_to_list ∘ vapply fl.
+Proof. elim fl; [done|]=>/= ??? Eq. fun_ext=>/= ?. by rewrite Eq. Qed.
+
 Lemma vapply_lookup {A B n} (fl: _ (B → A) n) (i: fin n) :
   (.!!! i) ∘ vapply fl = fl !!! i.
 Proof. by induction fl; inv_fin i. Qed.
